compiler/src/compilerExamples/SoftmulCompile.v
@@ -8,6 +8,7 @@ Require Import riscv.Utility.RegisterNames.
 Require riscv.Spec.PseudoInstructions.
 Require riscv.Utility.InstructionCoercions.
 Require Import riscv.Spec.Decode.
+Require riscv.Spec.Execute.
 Require Import riscv.Spec.Machine.
 Require Import riscv.Platform.Memory.
 Require Import riscv.Spec.CSRFile.
@@ -21,13 +22,29 @@ Require Import riscv.Utility.runsToNonDet.
 Require Import compiler.SeparationLogic.
 Require Import bedrock2.Syntax.
 Require Import bedrock2.ZnWords.
-Require Import riscv.Platform.Run.
 Require Import riscv.Utility.Encode.
 Require Import riscv.Proofs.EncodeBound.
 Require Import riscv.Platform.MinimalCSRs.
 Require Import riscv.Platform.MaterializeRiscvProgram.
 Require Import compiler.regs_initialized.
 Require Import bedrock2.SepAutoArray bedrock2.SepAuto.
+
+Open Scope bool_scope.
+
+(* like (decode RV32I), but additionally also accepts the Mul instruction
+   (but no other instructions from the M extension) *)
+Definition mdecode(inst: Z): Instruction :=
+  let opcode := bitSlice inst 0 7 in
+  let rd := bitSlice inst 7 12 in
+  let funct3 := bitSlice inst 12 15 in
+  let rs1 := bitSlice inst 15 20 in
+  let rs2 := bitSlice inst 20 25 in
+  let funct7 := bitSlice inst 25 32 in
+  if (opcode =? opcode_OP) && (funct3 =? funct3_MUL) && (funct7 =? funct7_MUL)
+  then MInstruction (Mul rd rs1 rs2)
+  else decode RV32I inst.
+
+Definition idecode: Z -> Instruction := decode RV32I.
 
 Section Riscv.
   Context {word: Word.Interface.word 32}.
@@ -50,13 +67,19 @@ Section Riscv.
 
   Local Hint Mode map.map - - : typeclass_instances.
 
-  Definition instr(iset: InstructionSet)(inst: Instruction)(addr: word): Mem -> Prop :=
+  Definition run1(decoder: Z -> Instruction): M unit :=
+    pc <- getPC;
+    inst <- Machine.loadWord Fetch pc;
+    Execute.execute (decoder (LittleEndian.combine 4 inst));;
+    endCycleNormal.
+
+  Definition instr(decoder: Z -> Instruction)(inst: Instruction)(addr: word): Mem -> Prop :=
     ex1 (fun z => sep (addr |-> truncated_scalar access_size.four z)
-                      (emp (decode iset z = inst /\ 0 <= z < 2 ^ 32))).
+                      (emp (decoder z = inst /\ 0 <= z < 2 ^ 32))).
 
   Declare Scope array_abbrevs_scope.
   Open Scope array_abbrevs_scope.
-  Notation "'program' iset" := (array (instr iset) 4) (at level 10): array_abbrevs_scope.
+  Notation "'program' d" := (array (instr d) 4) (at level 10): array_abbrevs_scope.
 
   (* both the finish-postcondition and the abort-postcondition are set to `post`
      to make sure `post` holds in all cases: *)
@@ -98,28 +121,56 @@ Section Riscv.
     Add s3 s3 sp           ; (* s3 := s3 + stack_start                                    *)
     Lw a1 s1 0             ; (* a1 := stack[s1]                                           *)
     Lw a2 s2 0               (* a2 := stack[s2]                                           *)
-  ]] ++ softmul_insts ++ [[          (* a3 := softmul(a1,a2) *)
-    Sw s3 a3 0               (* stack[s3] := a3                *)
+  ]] ++ softmul_insts ++ [[  (* a3 := softmul(a1,a2)                                      *)
+    Sw s3 a3 0;              (* stack[s3] := a3                                           *)
+    Jalr zero ra 0           (* return;                                                   *)
   ]].
 
   (* update if index is nonzero *)
   Definition updNz{A: Type}(l: list A)(i: Z)(v: A): list A :=
     if Z.eqb i 0 then l else List.upd l (Z.to_nat i) v.
 
-  Lemma mul_correct: forall initial a_regs (regvals: list word) invalidIInst R,
+  (* TODO will need some stack space *)
+  Lemma mul_correct: forall initial a_regs regvals invalidIInst R (post: State -> Prop)
+                            ret_addr sp_val rd rs1 rs2,
       initial.(nextPc) = word.add initial.(pc) (word.of_Z 4) ->
-      map.get initial.(regs) RegisterNames.a0 = Some a_regs ->
-      map.get initial.(regs) RegisterNames.a1 = Some invalidIInst ->
-      seps [a_regs |-> word_array regvals; initial.(pc) |-> program RV32I mul_insts; R]
-           initial.(mem) ->
-      runsTo (mcomp_sat (run1 RV32I)) initial (fun final =>
+      map.get initial.(regs) RegisterNames.a0 = Some (word.of_Z invalidIInst) ->
+      map.get initial.(regs) RegisterNames.a1 = Some a_regs ->
+      map.get initial.(regs) RegisterNames.ra = Some ret_addr ->
+      map.get initial.(regs) RegisterNames.sp = Some sp_val ->
+      mdecode invalidIInst = MInstruction (Mul rd rs1 rs2) ->
+      seps [a_regs |-> word_array regvals; initial.(pc) |-> program idecode mul_insts; R]
+           initial.(mem) /\
+      (forall newMem newRegs,
+        seps [a_regs |-> word_array (updNz regvals rd (word.mul
+                   (List.nth (Z.to_nat rs1) regvals default)
+                   (List.nth (Z.to_nat rs2) regvals default)));
+               initial.(pc) |-> program idecode mul_insts; R] newMem ->
+        map.get newRegs RegisterNames.sp = Some sp_val ->
+        post { initial with pc := ret_addr;
+                            nextPc := word.add ret_addr (word.of_Z 4);
+                            mem := newMem;
+                            regs := newRegs (* <- regs arbitrarily changed except sp *)
+                            (* log and csrs remain the same *) }) ->
+      runsTo (mcomp_sat (run1 idecode)) initial post.
+  Admitted.
+
+  (* Needed if the handler wants to handle the case where the instruction is not
+     a multiplication: *)
+  Lemma mul_correct_2: forall initial a_regs regvals invalidIInst R (post: State -> Prop),
+      initial.(nextPc) = word.add initial.(pc) (word.of_Z 4) ->
+      map.get initial.(regs) RegisterNames.a0 = Some invalidIInst ->
+      map.get initial.(regs) RegisterNames.a1 = Some a_regs ->
+      seps [a_regs |-> word_array regvals; initial.(pc) |-> program idecode mul_insts; R]
+           initial.(mem) /\
+      (forall final,
         ((* case 1: It was not the Mul instruction *)
          (map.get final.(regs) RegisterNames.a0 = Some (word.of_Z 0) /\
           (forall rd rs1 rs2, decode RV32IM (word.unsigned invalidIInst) <>
                                 MInstruction (Mul rd rs1 rs2)) /\
           seps [a_regs |-> word_array regvals;
-                initial.(pc) |-> program RV32I mul_insts; R] final.(mem)) \/
-         (* case 2: It was the Mul instruction *)
+                initial.(pc) |-> program idecode mul_insts; R] final.(mem))
+         \/ (* case 2: It was the Mul instruction *)
          (exists ans rd rs1 rs2 v1 v2,
           map.get final.(regs) RegisterNames.a0 = Some ans /\
           word.unsigned ans <> 0 /\
@@ -127,10 +178,12 @@ Section Riscv.
           nth_error regvals (Z.to_nat rs1) = Some v1 /\
           nth_error regvals (Z.to_nat rs2) = Some v2 /\
           seps [a_regs |-> word_array (updNz regvals rd (word.mul v1 v2));
-               initial.(pc) |-> program RV32I mul_insts; R] final.(mem))) /\
+               initial.(pc) |-> program idecode mul_insts; R] final.(mem))) ->
         (* In common: *)
         final.(pc) = word.add initial.(pc) (word.mul (word.of_Z 4)
-                           (word.of_Z (Z.of_nat (List.length mul_insts)))) /\
-        final.(nextPc) = word.add final.(pc) (word.of_Z 4)).
+                           (word.of_Z (Z.of_nat (List.length mul_insts)))) ->
+        final.(nextPc) = word.add final.(pc) (word.of_Z 4) ->
+        post final) ->
+      runsTo (mcomp_sat (run1 idecode)) initial post.
   Admitted.
 End Riscv.
